replace ff_exp by low-level pow2/pow3

aes/verif_gen_tables_LL.v
@@ -1,7 +1,71 @@
 Require Import floyd.proofauto.
 Require Import floyd.reassoc_seq.
 Require Import aes.aes.
-Require Import aes.tablesLL.
+
+Fixpoint repeat_op_nat{T: Type}(n: nat)(start: T)(op: T -> T): T := match n with
+| O => start
+| S m => op (repeat_op_nat m start op)
+end.
+
+Definition repeat_op{T: Type}(n: Z)(start: T)(op: T -> T): T := repeat_op_nat (Z.to_nat n) start op.
+
+Lemma repeat_op_step: forall {T: Type} (i: Z) (start: T) (op: T -> T),
+  0 <= i ->
+  repeat_op (i + 1) start op = op (repeat_op i start op).
+Proof.
+  intros. unfold repeat_op. rewrite Z2Nat.inj_add by omega.
+  rewrite Nat.add_1_r. simpl. reflexivity.
+Qed.
+
+Fixpoint repeat_op_table_nat{T: Type}(n: nat)(start: T)(op: T -> T): list T := match n with
+| O => []
+| S m => (repeat_op_table_nat m start op) ++ [repeat_op_nat m start op]
+end.
+
+Definition repeat_op_table{T: Type}(n: Z)(start: T)(op: T -> T): list T :=
+  repeat_op_table_nat (Z.to_nat n) start op.
+
+Lemma repeat_op_table_step: forall {T: Type} (i: Z) (start: T) (op: T -> T),
+  0 <= i ->
+  repeat_op_table (i + 1) start op = (repeat_op_table i start op) ++ [repeat_op i start op].
+Proof.
+  intros. unfold repeat_op_table. rewrite Z2Nat.inj_add by omega.
+  rewrite Nat.add_1_r. simpl. reflexivity.
+Qed.
+
+Definition times3(x: int): int := 
+  Int.and
+    (Int.xor x (Int.xor (Int.shl x (Int.repr 1))
+                        (if Int.eq (Int.and x (Int.repr 128)) Int.zero then Int.zero else Int.repr 27)))
+    (Int.repr 255).
+
+Definition pow3(e: Z): int := repeat_op e (Int.repr 1) times3.
+
+Definition times2(x: int): int := 
+  Int.and
+    (Int.xor (Int.shl x (Int.repr 1))
+             (if Int.eq (Int.and x (Int.repr 128)) Int.zero then Int.zero else Int.repr 27))
+    (Int.repr 255).
+
+Definition pow2(e: Z): int := repeat_op e (Int.repr 1) times2.
+
+(* instead of
+     Require Import aes.tablesLL.
+   we do, for the moment:
+*)
+Definition FSb := (@nil int).
+Definition FT0 := (@nil int).
+Definition FT1 := (@nil int).
+Definition FT2 := (@nil int).
+Definition FT3 := (@nil int).
+Definition RSb := (@nil int).
+Definition RT0 := (@nil int).
+Definition RT1 := (@nil int).
+Definition RT2 := (@nil int).
+Definition RT3 := (@nil int).
+Definition RCON := repeat_op_table 10 Int.one times2.
+
+Global Opaque FSb FT0 FT1 FT2 FT3 RSb RT0 RT1 RT2 RT3 RCON.
 
 Local Open Scope logic.
 
@@ -17,7 +81,12 @@ Definition tables_initialized (tables : val) := data_at Ews t_struct_tables (map
   (map Vint RT0, (map Vint RT1, (map Vint RT2, (map Vint RT3, 
   (map Vint RCON))))))))))) tables.
 
-Definition tables_uninitialized tables := data_at_ Ews t_struct_tables tables.
+Definition Vundef256 : list val := repeat Vundef 256%nat.
+
+Definition tables_uninitialized tables := data_at Ews t_struct_tables (Vundef256, 
+  (Vundef256, (Vundef256, (Vundef256, (Vundef256, (Vundef256,
+  (Vundef256, (Vundef256, (Vundef256, (Vundef256, 
+  (repeat Vundef 10))))))))))) tables.
 
 Definition gen_tables_spec :=
   DECLARE _aes_gen_tables
@@ -34,13 +103,6 @@ Definition gen_tables_spec :=
 
 Definition Gprog : funspecs := ltac:(with_library prog [ gen_tables_spec ]).
 
-Lemma ff_exp_range: forall a b,
-  0 <= a < 256 ->
-  0 <= b < 256 ->
-  0 <= Int.unsigned (ff_exp (Int.repr a) (Int.repr b)) < 256.
-Proof.
-Admitted.
-
 (* Calls forward_if with the current precondition to which the provided conditions are added *)
 (* QQQ TODO does this already exist? Add to library? *)
 Ltac forward_if_diff add := match add with
@@ -54,6 +116,20 @@ Ltac forward_if_diff add := match add with
   end
 end.
 
+Lemma pow2_range: forall e,
+  0 <= e ->
+  0 <= Int.unsigned (pow2 e) < 256.
+Admitted.
+
+Lemma pow3_range: forall e,
+  0 <= e ->
+  0 <= Int.unsigned (pow3 e) < 256.
+Admitted.
+
+Lemma pow3_inj: forall (i j : Z),
+  pow3 i = pow3 j -> Int.eqmod 255 i j.
+Admitted.
+
 Lemma body_gen_tables: semax_body Vprog Gprog f_aes_gen_tables gen_tables_spec.
 Proof.
   start_function.
@@ -62,7 +138,7 @@ Proof.
   forward_for_simple_bound 256 (EX i: Z,
     PROP ( 0 <= i ) (* TODO floyd: why do we only get "Int.min_signed <= i < 256", instead of lo=0 ?
                        Probably because there are 2 initialisations in the for-loop... *)
-    LOCAL (temp _x (Vint (ff_exp (Int.repr 3) (Int.repr i))); 
+    LOCAL (temp _x (Vint (pow3 i)); 
         (* TODO documentation should say that I don't need to do this *)
         (* TODO floyd: tactic should tell me so *)
         (* temp _i (Vint (Int.repr i)); *)
@@ -76,11 +152,11 @@ Proof.
               And btw, log[0] remains Vundef.
               Think "each j has to be stored in the right cell of the log array". *)
            !!(forall j, 1 <= j < i -> Vint (Int.repr j)
-                = Znth (Int.unsigned (ff_exp (Int.repr 3) (Int.repr j))) log Vundef)
+                = Znth (Int.unsigned (pow3 j)) log Vundef)
            && data_at Tsh (tarray tint 256) log lvar1;
          EX pow : list val,
            !!(Zlength pow = 256) &&
-           !!(forall j, 0 <= j < i -> Znth j pow Vundef = Vint (ff_exp (Int.repr 3) (Int.repr j)))
+           !!(forall j, 0 <= j < i -> Znth j pow Vundef = Vint (pow3 j))
            && data_at Tsh (tarray tint 256) pow lvar0;
          tables_uninitialized tables)).
   { (* init *)
@@ -97,10 +173,10 @@ Proof.
        TODO floyd: error message should say that I have to thaw *)
     thaw Fr.
     forward.
-    + entailer!. apply ff_exp_range; omega.
+    + entailer!. apply pow3_range; omega.
     + (* t'1 = ( x & 0x80 ) ? 0x1B : 0x00 ) *)
       forward_if_diff (PROP () LOCAL (temp _t'1 (Vint (
-        if Int.eq (Int.and (ff_exp (Int.repr 3) (Int.repr i)) (Int.repr 128)) Int.zero
+        if Int.eq (Int.and (pow3 i) (Int.repr 128)) Int.zero
         then Int.zero
         else (Int.repr 27)
       ))) SEP ()).
@@ -117,40 +193,58 @@ Proof.
         (* x = (x ^ ((x << 1) ^ t'1)) & 0xFF *)
         forward.
         entailer!.
-        { f_equal. admit. }
-        { Exists (upd_Znth i pow (Vint (ff_exp (Int.repr 3) (Int.repr i)))).
-          Exists (upd_Znth (Int.unsigned (ff_exp (Int.repr 3) (Int.repr i))) log (Vint (Int.repr i))).
+        { f_equal. unfold pow3. rewrite repeat_op_step by omega. reflexivity. }
+        { Exists (upd_Znth i pow (Vint (pow3 i))).
+          Exists (upd_Znth (Int.unsigned (pow3 i)) log (Vint (Int.repr i))).
           entailer!. assert (0 <= i < 256) by omega. repeat split.
           - replace 256 with (Zlength log) by assumption.
             apply upd_Znth_Zlength.
             replace (Zlength log) with 256 by assumption.
-            apply ff_exp_range; omega.
-          - (*  apply log_table_invariant; assumption. *) admit.
+            apply pow3_range; omega.
+          - intros. assert (1 <= j < i \/ j = i) as C by omega. destruct C as [C | C].
+            * rewrite upd_Znth_diff.
+              + auto.
+              + replace (Zlength log) with 256 by assumption. apply pow3_range; omega.
+              + replace (Zlength log) with 256 by assumption. apply pow3_range; omega.
+              + intro E. apply unsigned_eq_eq in E.
+                apply pow3_inj in E. unfold Int.eqmod in E. destruct E as [k E]. omega.
+            * subst. rewrite upd_Znth_same.
+              + reflexivity.
+              + replace (Zlength log) with 256 by assumption. apply pow3_range; omega.
           - replace 256 with (Zlength pow) by assumption.
             apply upd_Znth_Zlength. omega.
-          - (* apply pow_table_invariant; assumption. *) admit.
+          - intros. assert (0 <= j < i \/ j = i) as C by omega. destruct C as [C | C].
+            * rewrite upd_Znth_diff by omega. auto.
+            * subst. rewrite upd_Znth_same by omega. reflexivity.
         }
   } {
   Intros log pow.
 
+  unfold tables_uninitialized.
+  unfold_data_at 3%nat.
+  freeze [0; 1; 2; 3; 4; 5; 6; 7; 8; 9; 10; 11] Fr.
+
   (* next part: round constants *)
   forward_for_simple_bound 10 (EX i: Z,
-    (PROP ( 0 <= i ) (* note: the upper bound is added by the tactic, but the lower isn't! *)
-     LOCAL (temp _x (Vint (ff_exp (Int.repr 2) (Int.repr i)));
+     PROP ( 0 <= i ) (* note: the upper bound is added by the tactic, but the lower isn't! *)
+     LOCAL (temp _x (Vint (pow2 i));
             lvar _log (tarray tint 256) lvar1;
             lvar _pow (tarray tint 256) lvar0;
             gvar _tables tables)
-     SEP (data_at Tsh (tarray tint 256) log lvar1;
-          data_at Tsh (tarray tint 256) pow lvar0;
-          tables_uninitialized tables))).
+     SEP (field_at Ews t_struct_tables [StructField _RCON]
+                   ((map Vint (repeat_op_table i Int.one times2)) ++ (repeat_op_table (10-i) Vundef id))
+                   tables)). (* TODO why doesn't this typecheck? *)
   { (* init *)
-    forward. forward. Exists 0. entailer!. }
+    forward. forward. Exists 0. entailer!. Exists (repeat Vundef 10%nat). entailer!.
+    - intros. omega.
+    - apply d
+ }
   { (* body *)
     unfold tables_uninitialized.
+    unfold_data_at 3%nat.
     (* TODO floyd: if I don't unfold, "forward" fails with the default error message *)
+    freeze [0; 1; 2; 3; 4; 5; 6; 7; 8; 9; 10; 11] Fr.
     forward. entailer!.
-    simpl (field_at _ _ _ _ tables).
-    freeze [0; 1; 2] Fr.
     (* t'2 = ( x & 0x80 ) ? 0x1B : 0x00 ) *)
     forward_if_diff (PROP () LOCAL (temp _t'2 (Vint (
       if Int.eq (Int.and (ff_exp (Int.repr 2) (Int.repr i)) (Int.repr 128)) Int.zero
@@ -170,7 +264,7 @@ Proof.
       (* x = ((x << 1) ^ t'2)) & 0xFF *)
       forward.
       entailer!.
-      { (*
+      { f_equal. (*
 Vint (ff_exp (Int.repr 2) (Int.repr (i + 1))) =
 Vint
   (Int.and
